with Aymeric and Denis, a two-phase tactic for frame_delta (still with an admit)

examples/lowstar_permissions/Test.Array.fst
@@ -8,8 +8,8 @@ module R = LowStar.Resource
 module HST = FStar.HyperStack.ST
 
 
-#reset-options "--z3rlimit 5 --max_fuel 0 --max_ifuel 0 --z3cliopt smt.qi.eager_threshold=1000"
-
+#reset-options "--z3rlimit 10 --max_fuel 0 --max_ifuel 0 --z3cliopt smt.qi.eager_threshold=1000"
+#restart-solver
 let read_write_without_sharing () : RST.RST unit
   (R.empty_resource)
   (fun _ -> R.empty_resource)
@@ -52,6 +52,7 @@ let read_write_without_sharing () : RST.RST unit
   A.free b;
   ()
 
+#set-options "--warn_error '-271-296'"
 let read_write_with_sharing () : RST.RST unit
   (R.empty_resource)
   (fun _ -> R.empty_resource)
@@ -68,55 +69,63 @@ let read_write_with_sharing () : RST.RST unit
   let x1 =
     RST.rst_frame
       (R.(A.array_resource b <*> A.array_resource b1))
-      #(A.array_resource b)
-      (fun _ -> R.(A.array_resource b <*> A.array_resource b1))
-      #(fun _ -> A.array_resource b)
-      #(A.array_resource b1)
+      // #(A.array_resource b)
+        (fun _ -> R.(A.array_resource b <*> A.array_resource b1))
+      // #(fun _ -> A.array_resource b)
+      // #(A.array_resource b1)
       (fun _ ->
         A.index b 0ul
       )
   in
+  (* (R.(A.array_resource b <*> A.array_resource b1)) *)
   let b_first, b_second = RST.rst_frame
     (R.(A.array_resource b <*> A.array_resource b1))
-    #(A.array_resource b)
-    (fun (b_first, b_second) -> R.(A.array_resource b_first <*> A.array_resource b_second <*> A.array_resource b1))
-    #(fun (b_first, b_second) -> R.(A.array_resource b_first <*> A.array_resource b_second))
-    #(A.array_resource b1)
+    // #(A.array_resource b)
+    (fun p -> R.(A.array_resource (fst p) <*> A.array_resource (snd p) <*> A.array_resource b1))
+    // #(fun p -> R.(A.array_resource (fst p) <*> A.array_resource (snd p)))
+//    #(A.array_resource b1)
     (let f = fun _ -> A.split #FStar.UInt32.t b 1ul in f) //TODO: remove let binding
   in
+  (* R.(A.array_resource b_first <*> A.array_resource b_second <*> A.array_resource b1)  *)
   let h = HST.get () in
   assert((R.sel (A.array_view b_first) h).A.p = 0.5R);
   assert((R.sel (A.array_view b_second) h).A.p = 0.5R);
-  assume(R.inv R.(A.array_resource b_second <*> (A.array_resource b_first <*> A.array_resource b1)) h);
-  assume(RST.rst_inv R.(A.array_resource b_second <*> (A.array_resource b_first <*> A.array_resource b1)) h);
+  assert(R.inv R.(A.array_resource b_first <*> A.array_resource b_second <*> A.array_resource b1) h);
+  // admit()
+
+  // assume(R.inv R.(A.array_resource b_second <*> (A.array_resource b_first <*> A.array_resource b1)) h);
+  // assume(RST.rst_inv R.(A.array_resource b_second <*> (A.array_resource b_first <*> A.array_resource b1)) h);
+  // admit()
   let x2 = RST.rst_frame
-    (R.(A.array_resource b_second <*> (A.array_resource b_first <*> A.array_resource b1)))
-    #(A.array_resource b_second)
-    (fun _ -> R.(A.array_resource b_second <*> (A.array_resource b_first <*> A.array_resource b1)))
-    #(fun _ -> A.array_resource b_second)
-    #(R.(A.array_resource b_first <*> A.array_resource b1))
+    (R.(A.array_resource b_first <*> A.array_resource b_second <*> A.array_resource b1))
+    //(R.(A.array_resource b_second <*> (A.array_resource b_first <*> A.array_resource b1)))
+    // #(A.array_resource b_second)
+    (fun _ -> (R.(A.array_resource b_first <*> A.array_resource b_second <*> A.array_resource b1)))
+    //(fun _ -> R.(A.array_resource b_second <*> (A.array_resource b_first <*> A.array_resource b1)))
+    // #(fun _ -> A.array_resource b_second)
+//    #(R.(A.array_resource b_first <*> A.array_resource b1))
     (fun _ -> A.index b_second 0ul)
   in
+
   let h = HST.get () in
-  assume(R.inv R.(A.array_resource b_first <*> A.array_resource b_second <*> A.array_resource b1) h);
-  assume(RST.rst_inv R.(A.array_resource b_first <*> A.array_resource b_second <*> A.array_resource b1) h);
+  // assume(R.inv R.(A.array_resource b_first <*> A.array_resource b_second <*> A.array_resource b1) h);
+  // assume(RST.rst_inv R.(A.array_resource b_first <*> A.array_resource b_second <*> A.array_resource b1) h);
   assume((R.sel (A.array_view b_first) h).A.p = 0.5R);
   assume((R.sel (A.array_view b_second) h).A.p = 0.5R);
   let b = RST.rst_frame
     (R.(A.array_resource b_first <*> A.array_resource b_second <*> A.array_resource b1))
-    #(R.(A.array_resource b_first <*> A.array_resource b_second))
+    // #(R.(A.array_resource b_first <*> A.array_resource b_second))
     (fun b -> R.(A.array_resource b <*> A.array_resource b1))
-    #(fun b -> A.array_resource b)
-    #(A.array_resource b1)
+    // #(fun b -> A.array_resource b)
+    // #(A.array_resource b1)
     (fun _ -> A.glue b_first b_second)
   in
   let h = HST.get () in
+
   assume((R.sel (A.array_view b) h).A.p = 0.5R);
   assume((R.sel (A.array_view b1) h).A.p = 0.5R);
   assume(Arr.mergeable b b1 /\ Arr.freeable b); // These ones have to be fixed in Lowstar.Array
   A.merge b b1;
   let h = HST.get () in
   assert((R.sel (A.array_view b) h).A.p = 1.0R);
-  A.free b;
-  let h1 = HST.get () in
-  assume (RST.modifies (R.empty_resource) (R.empty_resource) h0 h1)
+  A.free b
